deps/poulet4/lib/Typed.v
@@ -115,3 +115,143 @@ Section Typed.
   | ExprCxConstant.
 
 End Typed.
+
+Require Import Coq.Lists.List.
+Import ListNotations.
+Require Poulet4.P4cub.Util.EquivUtil.
+
+Section P4TypeInd.
+  Variable tags_t : Type.
+
+  Notation typ := (@P4Type tags_t).
+  Notation ctrltyp := (@ControlType tags_t).
+  Notation funtyp := (@FunctionType tags_t).
+  Notation param := (@P4Parameter tags_t).
+
+  Variables (P : typ -> Prop) (Q : ctrltyp -> Prop) (R : funtyp -> Prop) (S : param -> Prop).
+  
+  Hypothesis HBool : P TypBool.
+  Hypothesis HStr : P TypString.
+  Hypothesis HInteger : P TypInteger.
+  Hypothesis HInt : forall w, P (TypInt w).
+  Hypothesis HBit : forall w, P (TypBit w).
+  Hypothesis HVarbit : forall w, P (TypVarBit w).
+  Hypothesis HArray : forall t n, P t -> P (TypArray t n).
+  Hypothesis HTuple : forall ts,
+      Forall P ts -> P (TypTuple ts).
+  Hypothesis HList : forall ts,
+      Forall P ts -> P (TypList ts).
+  Hypothesis HRecord : forall xts,
+      Forall (fun xt => P (snd xt)) xts -> P (TypRecord xts).
+  Hypothesis HSet : forall t, P t -> P (TypSet t).
+  Hypothesis HError : P TypError.
+  Hypothesis HMatchkind : P TypMatchKind.
+  Hypothesis HVoid : P TypVoid.
+  Hypothesis HHeader : forall xts,
+      Forall (fun xt => P (snd xt)) xts -> P (TypHeader xts).
+  Hypothesis HUnion : forall xts,
+      Forall (fun xt => P (snd xt)) xts -> P (TypHeaderUnion xts).
+  Hypothesis HStruct : forall xts,
+      Forall (fun xt => P (snd xt)) xts -> P (TypStruct xts).
+  Hypothesis HEnum : forall X t ms,
+      EquivUtil.predop P t -> P (TypEnum X t ms).
+  Hypothesis HName : forall X, P (TypTypeName X).
+  Hypothesis HNew : forall X t,
+      P t -> P (TypNewType X t).
+  Hypothesis HControl : forall ct, Q ct -> P (TypControl ct).
+  Hypothesis HParser : forall ct, Q ct -> P (TypParser ct).
+  Hypothesis HExtern : forall X, P (TypExtern X).
+  Hypothesis HFunction : forall ft,
+      R ft -> P (TypFunction ft).
+  Hypothesis HAction : forall ds cs,
+      Forall S ds -> Forall S cs -> P (TypAction ds cs).
+  Hypothesis HTable : forall X, P (TypTable X).
+  Hypothesis HPackage : forall Xs ws ps,
+      Forall S ps -> P (TypPackage Xs ws ps).
+  Hypothesis HSpecialized : forall t ts,
+      Forall P ts -> P t -> P (TypSpecializedType t ts).
+  Hypothesis HConstructor : forall Xs ws ps t,
+      Forall S ps -> P t -> P (TypConstructor Xs ws ps t).
+  Hypothesis HControlType : forall Xs ps,
+      Forall S ps -> Q (MkControlType Xs ps).
+  Hypothesis HFunctionType : forall Xs ps k t,
+      Forall S ps -> P t -> R (MkFunctionType Xs ps k t).
+  Hypothesis HParam : forall b d t n x,
+      P t -> S (MkParameter b d t n x).
+
+  Fixpoint my_P4Type_ind (t : typ) : P t :=
+    let fix L ts : Forall P ts :=
+        match ts with
+        | []     => Forall_nil _
+        | t :: ts => Forall_cons t (my_P4Type_ind t) (L ts)
+        end in
+    let fix AL xts : Forall (fun xt => P (snd xt)) xts :=
+        match xts with
+        | []                  => Forall_nil _
+        | ((_,t) as xt) :: xts => Forall_cons xt (my_P4Type_ind t) (AL xts)
+        end in
+    let PO to : EquivUtil.predop P to :=
+        match to with
+        | Some t => EquivUtil.predop_some _ t (my_P4Type_ind t)
+        | None   => EquivUtil.predop_none _
+        end in
+    let fix PL ps : Forall S ps :=
+        match ps with
+        | []     => Forall_nil _
+        | p :: ps => Forall_cons p (my_P4Parameter_ind p) (PL ps)
+        end in
+    match t with
+    | TypBool      => HBool
+    | TypString    => HStr
+    | TypInteger   => HInteger
+    | TypInt w     => HInt w
+    | TypBit w     => HBit w
+    | TypVarBit w  => HVarbit w
+    | TypArray t n => HArray t n (my_P4Type_ind t)
+    | TypTuple ts  => HTuple ts (L ts)
+    | TypList  ts  => HList  ts (L ts)
+    | TypSet t     => HSet t (my_P4Type_ind t)
+    | TypError     => HError
+    | TypVoid      => HVoid
+    | TypMatchKind => HMatchkind
+    | TypRecord      ts => HRecord ts (AL ts)
+    | TypHeader      ts => HHeader ts (AL ts)
+    | TypHeaderUnion ts => HUnion  ts (AL ts)
+    | TypStruct      ts => HStruct ts (AL ts)
+    | TypEnum X t ms    => HEnum X t ms (PO t)
+    | TypTypeName X     => HName X
+    | TypNewType  X t   => HNew X t (my_P4Type_ind t)
+    | TypControl ct     => HControl ct (my_ControlType_ind ct)
+    | TypParser  ct     => HParser  ct (my_ControlType_ind ct)
+    | TypExtern  X      => HExtern X
+    | TypFunction ft    => HFunction ft (my_FunctionType_ind ft)
+    | TypAction ds cs   => HAction ds cs (PL ds) (PL cs)
+    | TypTable X        => HTable X
+    | TypPackage Xs ws ps       => HPackage Xs ws ps (PL ps)
+    | TypSpecializedType t ts   => HSpecialized t ts (L ts) (my_P4Type_ind t)
+    | TypConstructor Xs ws ps t => HConstructor Xs ws ps t (PL ps) (my_P4Type_ind t)
+    end
+  with my_ControlType_ind (ct : ctrltyp) : Q ct :=
+         let fix PL ps : Forall S ps :=
+             match ps with
+             | []     => Forall_nil _
+             | p :: ps => Forall_cons p (my_P4Parameter_ind p) (PL ps)
+             end in
+         match ct with
+         | MkControlType Xs ps => HControlType Xs ps (PL ps)
+         end
+  with my_FunctionType_ind (ft : funtyp) : R ft :=
+         let fix PL ps : Forall S ps :=
+             match ps with
+             | []     => Forall_nil _
+             | p :: ps => Forall_cons p (my_P4Parameter_ind p) (PL ps)
+             end in
+         match ft with
+         | MkFunctionType Xs ps k t
+           => HFunctionType Xs ps k t (PL ps) (my_P4Type_ind t)
+         end
+  with my_P4Parameter_ind (p : param) : S p :=
+         match p with
+         | MkParameter b d t n x => HParam b d t n x (my_P4Type_ind t)
+         end.
+End P4TypeInd.
